test/artifact/pneutube/PaddedFileIO.fst
@@ -1,6 +1,8 @@
 module PaddedFileIO
 
 open FStar.Seq
+open FStar.HyperHeap
+open FStar.HyperStack
 open FStar.Buffer
 open Hacl.Cast
 open Hacl.Constants
@@ -13,6 +15,12 @@ module H32 =  Hacl.UInt32
 module U64 = FStar.UInt64
 module H64 =  Hacl.UInt64
 module B   = FStar.Buffer
+module HS  = FStar.HyperStack
+module HH  = FStar.HyperHeap
+
+assume val file_rgn: r:rid{is_eternal_region r}
+type fh_ref = fb:buffer file_handle{length fb = 1 /\ frameOf fb = file_rgn}
+
 
 #reset-options "--initial_fuel 0 --max_fuel 0"
 private val lemma_max_uint8: n:nat -> Lemma
@@ -31,80 +39,81 @@ private val lemma_max_uint64: n:nat -> Lemma
  [SMTPat (pow2 n)]
 let lemma_max_uint64 n = assert_norm(pow2 64 = 18446744073709551616)
 
-(* Need to get rid of these  following ones *)
-type string = seq u8
-
 inline_for_extraction val zero: u64
 inline_for_extraction let zero = 0uL
-(* The above need to come from some library module *)
-
-type bufsize = x:U64.t{U64.v x < pow2 32}
-
-private let bufsize_bound (x:bufsize) : Lemma (requires (True)) (ensures (U32.v (Int.Cast.uint64_to_uint32 x) = U64.v x)) [SMTPat (Int.Cast.uint64_to_uint32 x)] = Math.Lemmas.modulo_lemma (U64.v x) (pow2 32)
 
 (* File System Buffer Size, currently 256KB *)
 inline_for_extraction val max_block_size: u64
 inline_for_extraction let max_block_size = 262144uL
 
+type bufsize = x:U64.t{U64.v x < pow2 32}
 
-assume val file_state: FStar.HyperStack.mem -> file_handle -> GTot fd_state
-assume val file_offset: FStar.HyperStack.mem -> file_handle -> GTot u64
-assume val file_buffer: FStar.HyperStack.mem -> file_stat -> GTot (buffer h8)
+private let bufsize_bound (x:bufsize) : Lemma (requires (True)) (ensures (U32.v (Int.Cast.uint64_to_uint32 x) = U64.v x)) [SMTPat (Int.Cast.uint64_to_uint32 x)] = Math.Lemmas.modulo_lemma (U64.v x) (pow2 32)
 
-let file_sub (m:FStar.HyperStack.mem) (f:file_handle) (i:u64) (j:u64{U64.v j + U64.v i <= length (file_buffer m f.stat)}) =
-    B.sub (file_buffer m f.stat) (Int.Cast.uint64_to_uint32 i) (Int.Cast.uint64_to_uint32 j)
+
+assume val file_state_: FStar.Heap.heap -> file_handle -> GTot fd_state
+let file_state (h:mem) fh : GTot fd_state = file_state_ (Map.sel h.h file_rgn) fh
+assume val file_offset_: FStar.Heap.heap -> file_handle -> GTot u64
+let file_offset (h:mem) fh : GTot u64 = file_offset_ (Map.sel h.h file_rgn) fh
+assume val file_buffer: file_stat -> GTot (buffer h8)
+
+let file_sub (m:FStar.HyperStack.mem) (f:file_handle) (i:u64) (j:u64{U64.v j + U64.v i <= length (file_buffer f.stat)}) =
+    B.sub (file_buffer f.stat) (Int.Cast.uint64_to_uint32 i) (Int.Cast.uint64_to_uint32 j)
 
 
 (* A live file handle maps to a buffer which max_length is the size indicated in the file_stat *)
 let live_fh h (fh:file_handle) : GTot Type0 =
-  live h (file_buffer h fh.stat)
-  /\ max_length (file_buffer h fh.stat) = H64.v fh.stat.size
-  /\ length (file_buffer h fh.stat) = H64.v fh.stat.size
+  live h (file_buffer fh.stat)
+  /\ max_length (file_buffer fh.stat) = H64.v fh.stat.size
+  /\ length (file_buffer fh.stat) = H64.v fh.stat.size
   /\ U64.v (file_offset h fh) <= H64.v fh.stat.size
 
 (* Type of a workable file *)
-let live_file h (f:buffer file_handle) : GTot Type0 =
-  length f = 1 /\ live h f /\ (let fh = get h f 0 in live_fh h fh)
+let live_file h (f:fh_ref) : GTot Type0 =
+  live h f /\ (let fh = get h f 0 in live_fh h fh)
 
 (* Files are not changed through reads/writes *)
 let same_file h f h' f' : GTot Type0 =
   live_file h f /\ live_file h' f'
   /\ (let fh = get h f 0 in let fh' = get h' f' 0 in  fh.stat == fh'.stat)
 
-val file_content: h:FStar.HyperStack.mem -> fs:file_stat{live h (file_buffer h fs)}  -> GTot (seq h8)
-let file_content m fs = as_seq m (file_buffer m fs)
+val file_content: h:FStar.HyperStack.mem -> fs:file_stat{live h (file_buffer fs)}  -> GTot (seq h8)
+let file_content m fs = as_seq m (file_buffer fs)
 
 
 (* TODO: check the live/modifies clauses below *)
 assume val file_open_read_sequential: n:uint8_p ->
-  fb:buffer file_handle{disjoint n fb /\ length fb = 1} ->
+  fb:fh_ref ->
   Stack fresult
     (requires (fun h -> live h fb /\ live h n))
     (ensures  (fun h0 s h1 -> (match s with
 	      	       	    | FileOk ->
-			      modifies_1 fb h0 h1 /\
-                              live_file h1 fb /\
+			      (* modifies_1 fb h0 h1 /\ *)
+                              HS.modifies (Set.singleton file_rgn) h0 h1
+                              /\ live_file h1 fb /\
 			      (let fh = get h1 fb 0 in
     	      	     	       file_state h1 fh = FileOpen /\
 			       file_offset h1 fh = zero /\
-			       length (file_buffer h1 fh.stat) = max_length (file_buffer h1 fh.stat))
+			       length (file_buffer fh.stat) = max_length (file_buffer fh.stat))
 			       (* /\ file_content h0 fh.stat == file_content h1 fh.stat) *)
 			    | _ -> true)))
 
 
 assume val file_open_write_sequential: file_stat ->
-  fb:buffer file_handle{length fb = 1} ->
+  fb:fh_ref ->
   Stack fresult
     (requires (fun h -> live h fb))
     (ensures  (fun h0 s h1 -> match s with
     	      	      	    | FileOk ->
-			      live_file h1 fb /\
+                              HS.modifies (Set.singleton file_rgn) h0 h1
+			      /\ live_file h1 fb /\
 			      (let fh = get h1 fb 0 in
     	      	      	       file_state h1 fh = FileOpen /\
 			       file_offset h1 fh = zero /\
-			       length (file_buffer h1 fh.stat) = max_length (file_buffer h1 fh.stat))
+			       length (file_buffer fh.stat) = max_length (file_buffer fh.stat))
 			       (* file_content h0 fh.stat == file_content h1 fh.stat) *)
 			    | _ -> true))
+
 
 private let sint64_to_uint64 (x:H64.t) : GTot U64.t = U64.uint_to_t (H64.v x)
 private let sint64_to_uint32 (x:H64.t) : GTot U32.t = Int.Cast.uint64_to_uint32 (U64.uint_to_t (H64.v x))
@@ -128,46 +137,46 @@ private let sint64_to_uint32 (x:H64.t) : GTot U32.t = Int.Cast.uint64_to_uint32 
 (* 			      ((U64.v i <= v f.stat.size /\ H64.v j > v f.stat.size) ==> (B.sub s 0ul (sint64_to_uint32 ((f.stat.size -^ Hacl.Cast.uint64_to_sint64 i))) == file_sub h1 f i (sint64_to_uint64 (f.stat.size -^ Hacl.Cast.uint64_to_sint64 i)))) *)
 (*                               )) *)
 
-let file_next_read_buffer_pre h (fb:buffer file_handle{length fb = 1}) (len:U64.t) : GTot Type0 =
+let file_next_read_buffer_pre h (fb:fh_ref) (len:U64.t) : GTot Type0 =
   live_file h fb /\ U64.v len <= U64.v max_block_size
   /\ (let fh = get h fb 0 in file_state h fh = FileOpen
     /\ U64.v (file_offset h fh) + U64.v len <= H64.v fh.stat.size)
 
-let file_next_read_buffer_post h0 (s:uint8_p) h1 (fb:buffer file_handle{length fb = 1})
+let file_next_read_buffer_post h0 (s:uint8_p) h1 (fb:fh_ref{length fb = 1})
                                (len:bufsize) : GTot Type0 =
   file_next_read_buffer_pre h0 fb len
   /\ live_file h0 fb /\ live_file h1 fb /\ same_file h0 fb h1 fb
   /\ (let fh0 = get h0 fb 0 in let fh1 = get h1 fb 0 in
       U64.v (file_offset h1 fh1) = U64.v (file_offset h0 fh0) + U64.v len
       /\ file_state h1 fh1 = FileOpen
-      /\ s == Buffer.sub (file_buffer h0 fh0.stat) (Int.Cast.uint64_to_uint32 (file_offset h0 fh0)) (Int.Cast.uint64_to_uint32 len))
-  /\ modifies_1 fb h0 h1
+      /\ s == Buffer.sub (file_buffer fh0.stat) (Int.Cast.uint64_to_uint32 (file_offset h0 fh0)) (Int.Cast.uint64_to_uint32 len))
+  /\ HS.modifies (Set.singleton file_rgn) h0 h1
 
 
 assume val file_next_read_buffer:
-  fb:buffer file_handle{length fb = 1} ->
+  fb:fh_ref ->
   len:bufsize ->
   Stack uint8_p
     (requires (fun h0 -> file_next_read_buffer_pre h0 fb len))
     (ensures  (fun h0 s h1 -> file_next_read_buffer_post h0 s h1 fb len))
 
 
-let file_next_write_buffer_pre h (fb:buffer file_handle{length fb = 1}) (len:U64.t) : GTot Type0 =
+let file_next_write_buffer_pre h (fb:fh_ref) (len:U64.t) : GTot Type0 =
   live_file h fb /\ U64.v len <= U64.v max_block_size
   /\ (let fh = get h fb 0 in file_state h fh = FileOpen
     /\ U64.v (file_offset h fh) + U64.v len <= H64.v fh.stat.size)
 
-let file_next_write_buffer_post h0 (s:uint8_p) h1 (fb:buffer file_handle{length fb = 1})
+let file_next_write_buffer_post h0 (s:uint8_p) h1 (fb:fh_ref)
                                (len:bufsize) : GTot Type0 =
   file_next_read_buffer_pre h0 fb len
   /\ live_file h0 fb /\ live_file h1 fb /\ same_file h0 fb h1 fb
   /\ (let fh0 = get h0 fb 0 in let fh1 = get h1 fb 0 in
       U64.v (file_offset h1 fh1) = U64.v (file_offset h0 fh0) + U64.v len
       /\ file_state h1 fh1 = FileOpen
-      /\ s == Buffer.sub (file_buffer h0 fh0.stat) (Int.Cast.uint64_to_uint32 (file_offset h0 fh0)) (Int.Cast.uint64_to_uint32 len))
-  /\ modifies_1 fb h0 h1
+      /\ s == Buffer.sub (file_buffer fh0.stat) (Int.Cast.uint64_to_uint32 (file_offset h0 fh0)) (Int.Cast.uint64_to_uint32 len))
+  /\ HS.modifies (Set.singleton file_rgn) h0 h1
 
-assume val file_next_write_buffer: fb:buffer file_handle{length fb = 1} -> len:bufsize -> Stack uint8_p
+assume val file_next_write_buffer: fb:fh_ref -> len:bufsize -> Stack uint8_p
     (requires (fun h0 -> file_next_write_buffer_pre h0 fb len))
     (ensures  (fun h0 s h1 -> file_next_read_buffer_post h0 s h1 fb len))
 
@@ -188,10 +197,11 @@ assume val file_next_write_buffer: fb:buffer file_handle{length fb = 1} -> len:b
 (*                               )) *)
 
 
-assume val file_close: fb:buffer file_handle{length fb = 1} -> Stack bool
+assume val file_close: fb:fh_ref -> Stack bool
     (requires (fun h0 -> length fb = 1 /\ live_file h0 fb /\
                          (let f = get h0 fb 0 in
 			  file_state h0 f = FileOpen)))
     (ensures  (fun h0 r h1 -> live_file h0 fb /\ live_file h1 fb /\ same_file h0 fb h1 fb
+      /\ HS.modifies (Set.singleton file_rgn) h0 h1
       /\ (r ==> (let f = get h1 fb 0 in file_state h1 f = FileClosed /\
     			              file_content h0 f.stat == file_content h1 f.stat))))
